\documentclass{ximera}
\input{../preamble.tex}

\title{Exercises} \license{CC BY-NC-SA 4.0}

\begin{document}

\begin{abstract}
\end{abstract}
\maketitle

\begin{onlineOnly}
\section*{Exercises}
\end{onlineOnly}


\begin{problem}\label{exer:7.1.1}
\begin{enumerate}

\item Use Theorem~\ref{thmtype:7.1.3} to find the radius of convergence $R$. If $R>0$, find the open interval of convergence.

$\sum_{n=0}^\infty \frac{(-1)^n}{2^nn}(x-1)^n$

\item Use Theorem~\ref{thmtype:7.1.3} to find the radius of convergence $R$. If $R>0$, find the open interval of convergence.

$\sum_{n=0}^\infty 2^nn(x-2)^n$

\item Use Theorem~\ref{thmtype:7.1.3} to find the radius of convergence $R$. If $R>0$, find the open interval of convergence.
$\sum_{n=0}^\infty \frac{n!}{9^n}x^n$

\item Use Theorem~\ref{thmtype:7.1.3} to find the radius of convergence $R$. If $R>0$, find the open interval of convergence.

$\sum_{n=0}^\infty\frac{n(n+1)}{16^n}(x-2)^n$

\item Use Theorem~\ref{thmtype:7.1.3} to find the radius of convergence $R$. If $R>0$, find the open interval of convergence.

$\sum_{n=0}^\infty (-1)^n\frac{7^n}{n!}x^n$

\item Use Theorem~\ref{thmtype:7.1.3} to find the radius of convergence $R$. If $R>0$, find the open interval of convergence.

$\sum_{n=0}^\infty \frac{3^n}{4^{n+1}(n+1)^2}(x+7)^n$
\end{enumerate}
\end{problem}

\begin{problem}\label{exer:7.1.2}
Suppose there is an integer $M$ such that $b_m\ne0$ for $m\ge M$,  and
$$
\lim_{m\to\infty}\left|\frac{b_{m+1}}{b_m}\right|=L,
$$
where $0\le L\le\infty$. Show that the radius of convergence of
$$
\sum_{m=0}^\infty b_m(x-x_0)^{2m}
$$
is $R=1/\sqrt L$,
which is interpreted to mean that $R=0$ if $L=\infty$ or
$R=\infty$ if $L=0$.
\begin{hint}
 Apply Theorem~$\ref{thmtype:7.1.3}$ to the series $\sum_{m=0}^\infty
b_mz^m$ and then let $z=(x-x_0)^2$.   
\end{hint}

\begin{solution}
    From Theorem~\ref{thmtype:7.1.3}, $\sum_{m=0}^\infty b_mz^m$ converges
if $|z|<1/L$ and diverges if $|z|>1/L$.
 Therefore,
$\sum_{m=0}^\infty b_m(x-x_0)^2$ converges if $|x-x_0|<1/\sqrt{L}$
and diverges if $|x-x_0|>1/\sqrt{L}$.
\end{solution}
\end{problem}

\begin{problem}\label{exer:7.1.3}
\begin{enumerate}

\item Use the result of Exercise~\ref{exer:7.1.2} to find the radius of convergence $R$. If $R>0$, find the open interval of convergence.

$\sum_{m=0}^\infty (-1)^m(3m+1)(x-1)^{2m+1}$

\item Use the result of Exercise~\ref{exer:7.1.2} to find the radius of convergence $R$. If $R>0$, find the open interval of convergence.
$\sum_{m=0}^\infty (-1)^m\frac{m(2m+1)}{2^m}(x+2)^{2m}$ 

\item Use the result of Exercise~\ref{exer:7.1.2} to find the radius of convergence $R$. If $R>0$, find the open interval of convergence.
$\sum_{m=0}^\infty \frac{m!}{(2m)!}(x-1)^{2m}$

\item Use the result of Exercise~\ref{exer:7.1.2} to find the radius of convergence $R$. If $R>0$, find the open interval of convergence.
$\sum_{m=0}^\infty (-1)^m\frac{m!}{9^m}(x+8)^{2m}$

\item Use the result of Exercise~\ref{exer:7.1.2} to find the radius of convergence $R$. If $R>0$, find the open interval of convergence.
$\sum_{m=0}^\infty(-1)^m\frac{(2m-1)}{3^m}x^{2m+1}$

\item Use the result of Exercise~\ref{exer:7.1.2} to find the radius of convergence $R$. If $R>0$, find the open interval of convergence.
$\sum_{m=0}^\infty(x-1)^{2m}$

\end{enumerate}
\end{problem}

\begin{problem}\label{exer:7.1.4}
Suppose there is an integer $M$ such that $b_m\ne0$ for $m\ge M$,
and
$$
\lim_{m\to\infty}\left|\frac{b_{m+1}}{b_m}\right|=L,
$$
where $0\le L\le\infty$. Let $k$ be a positive integer. Show that the
radius of convergence of
$$
\sum_{m=0}^\infty b_m(x-x_0)^{km}
$$
is $R=1/\sqrt[k]L$, which is interpreted to mean that $R=0$ if
$L=\infty$ or $R=\infty$ if $L=0$.

\begin{hint}
Apply Theorem~$\ref{thmtype:7.1.3}$
to the series $\sum_{m=0}^\infty b_mz^m$ and then let $z=(x-x_0)^k$.    
\end{hint}

\begin{solution}
    From Theorem~7.1.3, $\sum_{m=0}^\infty b_mz^m$ converges
if $|z|<1/L$ and diverges if $|z|>1/L$.
 Therefore,
$\sum_{m=0}^\infty b_m(x-x_0)^{km}$ converges if
$|x-x_0|<1/\sqrt[k]{L}$ and diverges if $|x-x_0|>1/\sqrt[k]{L}$.
\end{solution}
\end{problem}

\begin{problem}\label{exer:7.1.5}

\begin{enumerate}
\item Use the result of Exercise~\ref{exer:7.1.4} to find the radius of convergence $R$. If $R>0$, find the open interval of convergence.
    
 $\sum_{m=0}^\infty\frac{(-1)^m}{(27)^m}(x-3)^{3m+2}$
 
\item Use the result of Exercise~\ref{exer:7.1.4} to find the radius of convergence $R$. If $R>0$, find the open interval of convergence.
 
 $\sum_{m=0}^\infty\frac{x^{7m+6}}{m}$ 
 
\item Use the result of Exercise~\ref{exer:7.1.4} to find the radius of convergence $R$. If $R>0$, find the open interval of convergence.
 
 $\sum_{m=0}^\infty\frac{9^m(m+1)}{(m+2)}(x-3)^{4m+2}$
 
\item Use the result of Exercise~\ref{exer:7.1.4} to find the radius of convergence $R$. If $R>0$, find the open interval of convergence.
 
 $\sum_{m=0}^\infty(-1)^m\frac{2^m}{m!}x^{4m+3}$
 
\item Use the result of Exercise~\ref{exer:7.1.4} to find the radius of convergence $R$. If $R>0$, find the open interval of convergence.
 
 $\sum_{m=0}^\infty\frac{m!}{(26)^m}(x+1)^{4m+3}$
 
\item Use the result of Exercise~\ref{exer:7.1.4} to find the radius of convergence $R$. If $R>0$, find the open interval of convergence.
 
 $\sum_{m=0}^\infty\frac{(-1)^m}{8^mm(m+1)}(x-1)^{3m+1}$
\end{enumerate}
\end{problem}

\begin{problem}\label{exer:7.1.6}  
Graph $y=\sin x$ and the Taylor polynomial
$$
T_{2M+1}(x)=\sum_{n=0}^M\frac{(-1)^nx^{2n+1}}{(2n+1)!}
$$
on the interval $(-2\pi,2\pi)$ for $M=1$, $2$, $3$, \dots, until you find
a value of $M$ for which there is no perceptible difference between the
two graphs.

\end{problem}


\begin{problem}\label{exer:7.1.7}  
Graph $y=\cos x$ and the Taylor polynomial
$$
T_{2M}(x)=\sum_{n=0}^M\frac{(-1)^nx^{2n}}{(2n)!}
$$
on the interval $(-2\pi,2\pi)$ for $M=1$, $2$, $3$, \dots, until you find a
value of $M$ for which there is no perceptible difference between the
two graphs.
\end{problem}

\begin{problem}\label{exer:7.1.8}  
Graph $y=1/(1-x)$ and the Taylor polynomial
$$
T_N(x)=\sum_{n=0}^Nx^n
$$
on the interval $[0,.95]$ for $N=1$, $2$, $3$, \dots, until you find a
value of $N$ for which there is no perceptible difference between the
two graphs. Choose the scale on the $y$-axis so that $0\le y\le20$.
\end{problem}

\begin{problem}\label{exer:7.1.9}  
Graph $y=\cosh x$ and the Taylor polynomial
$$
T_{2M}(x)=\sum_{n=0}^M\frac{x^{2n}}{(2n)!}
$$
on the interval $(-5,5)$ for $M=1$, $2$, $3$, \dots, until you find a
value of $M$ for which there is no perceptible difference between the
two graphs.
 Choose the scale on the $y$-axis so that $0\le y\le75$.
\end{problem}

\begin{problem}\label{exer:7.1.10}  
Graph $y=\sinh x$ and the Taylor polynomial
$$
T_{2M+1}(x)=\sum_{n=0}^M\frac{x^{2n+1}}{(2n+1)!}
$$
on the interval $(-5,5)$ for $M=0$, $1$, $2$, \dots, until you find a
value of $M$ for which there is no perceptible difference between the
two graphs.  Choose the scale on the $y$-axis so that~$-75~\le~y\le~75$.
 \end{problem}

\begin{problem}\label{exer:7.1.11}
Find a power series solution $y(x)=\sum_{n=0}^\infty a_nx^n$.

$(2+x)y''+xy'+3y$
\end{problem}

\begin{problem}\label{exer:7.1.12}
Find a power series solution $y(x)=\sum_{n=0}^\infty a_nx^n$.

$(1+3x^2)y''+3x^2y'-2y$

\begin{solution}
    $$(1+3x^2)y''+3x^2y'-2y=$$
$$=\sum_{n=2}^\infty n(n-1)a_nx^{n-2}
+3\sum_{n=2}^\infty n(n-1)a_nx^n
+3\sum_{n=1}^\infty na_nx^{n+1}-2\sum_{n=0}^\infty a_nx^n=$$
$$=\sum_{n=0}^\infty (n+2)(n+1)a_{n+2}x^n
+3\sum_{n=1}^\infty n(n-1)na_nx^n
+3\sum_{n=1}^\infty (n-1)a_{n-1}x^n-2\sum_{n=0}^\infty a_nx^n=$$
$$=2a_2-2a_0+\sum_{n=1}^\infty
[(n+2)(n+1)a_{n+2}+(3n(n-1)-2)a_n+3(n-1)a_{n-1}]x^n
$$
\end{solution}
\end{problem}

\begin{problem}\label{exer:7.1.13} 
Find a power series solution $y(x)=\sum_{n=0}^\infty a_nx^n$.

$(1+2x^2)y''+(2-3x)y'+4y$

%\begin{solution}
%    $$(1+2x^2)y''+(2-3x)y'+4y=$$
%    $$=
%\sum_{n=2}^\infty n(n-1)a_nx^{n-2}
%+2\sum_{n=2}^\infty n(n-1)a_nx^n
%+2\sum_{n=1}^\infty na_nx^{n-1}-2\sum_{n=0}^\infty a_nx^n
%+4\sum_{n=0}^\infty a_nx^n=$$
%$$=\sum_{n=0}^\infty (n+2)(n+1)a_{n+2}x^n
%+2\sum_{n=0}^\infty n(n-1)a_nx^n
%+2\sum_{n=0}^\infty (n+1)a_{n+1}x^n
%-3\sum_{n=0}^\infty a_nx^n
%+4\sum_{n=0}^\infty a_nx^n
%\sum_{n=0}^\infty
%\left[(n+2)(n+1)a_{n+2}+2(n+1)a_{n+1}+(2n^2-5n+4)a_n\right]x^n
%$$
%\end{solution}
\end{problem}

\begin{problem}\label{exer:7.1.14}
Find a power series solution $y(x)=\sum_{n=0}^\infty a_nx^n$.

$(1+x^2)y''+(2-x)y'+3y$

\begin{solution}
    $$(1+x^2)y''+(2-x)y'+3y=$$
$$=\sum_{n=2}^\infty n(n-1)a_nx^{n-2}
+\sum_{n=2}^\infty n(n-1)a_nx^n
+2\sum_{n=1}^\infty na_nx^{n-1}-\sum_{n=1}^\infty na_nx^n
+3\sum_{n=0}^\infty a_nx^n=$$
$$=\sum_{n=0}^\infty (n+2)(n+1)a_{n+2}x^n
+\sum_{n=0}^\infty n(n-1)a_nx^n
+2\sum_{n=0}^\infty (n+1)a_{n+1}x^n-\sum_{n=0}^\infty na_nx^n
+3\sum_{n=0}^\infty a_nx^n=$$
$$=\sum_{n=0}^\infty
\left[(n+2)(n+1)a_{n+2}+2(n+1)a_{n+1}+(n^2-2n+3)a_n\right]x^n
$$
\end{solution}
\end{problem}

\begin{problem}\label{exer:7.1.15}
Find a power series solution $y(x)=\sum_{n=0}^\infty a_nx^n$.

$(1+3x^2)y''-2xy'+4y$
\end{problem}

\begin{problem}\label{exer:7.1.16} Suppose $y(x)=\sum_{n=0}^\infty a_n(x+1)^n$
on an open interval that contains $x_0~=~-1$. Find a power series in
$x+1$ for
$$
xy''+(4+2x)y'+(2+x)y.
$$

\begin{solution}
    Let $t=x+1$; then 
    $$xy''+(4+2x)y'+(2+x)y=$$
    $$=(-1+t)y''+(2+2t)y'+(1+t)y=$$
$$=-\sum_{n=2}^\infty n(n-1)a_nt^{n-2}
+\sum_{n=2}^\infty n(n-1)a_nt^{n-1}
+2\sum_{n=1}^\infty n a_nt^{n-1}
+2\sum_{n=1}^\infty n a_nt^n
+\sum_{n=0}^\infty  a_nt^n
+\sum_{n=0}^\infty  a_nt^{n+1}=$$
$$=-\sum_{n=0}^\infty (n+2)(n+1)a_{n+2}t^n
+\sum_{n=0}^\infty (n+1)na_{n+1}t^n
+2\sum_{n=0}^\infty (n+1) a_{n+1}t^n
+2\sum_{n=0}^\infty n a_nt^n
+\sum_{n=0}^\infty  a_nt^n
+\sum_{n=1}^\infty  a_{n-1}t^n=$$
$$=(-2a_2+2a_1+a_0)
+\sum_{n=1}^\infty
 \left[-(n+2)(n+1)a_{n+2}+(n+1)(n+2)a_{n+1}+(2n+1)a_n+a_{n-1}\right]
(x+2)^n
$$
\end{solution}
\end{problem}

\begin{problem}\label{exer:7.1.17}  Suppose $y(x)=\sum_{n=0}^\infty
a_n(x-2)^n$ on an open interval  that contains $x_0~=~2$.
Find a power series in $x-2$ for
$$
x^2y''+2xy'-3xy.
$$
\end{problem}

\begin{problem}\label{exer:7.1.18}   
Do the following experiment for various choices of
real numbers  $a_0$ and $a_1$.
\begin{enumerate}
\item % (a)
Use software  to solve the initial value problem
$$
(2-x)y''+2y=0,\quad y(0)=a_0,\quad y'(0)=a_1,
$$
numerically on $(-1.95,1.95)$. Choose the most accurate method
your software provides.
(See Section~10.1 for a brief discussion of one such
method.)
\item % (b)
For $N=2$, $3$, $4$, \dots, compute $a_2$, \dots, $a_N$
from Eqn.\eqref{eq:7.1.18} and graph
$$
T_N(x)=\sum_{n=0}^N a_nx^n
$$
and the solution obtained above on the same axes.
Continue increasing $N$ until it is obvious that there is
no point in continuing.
(This sounds vague, but you will know when to stop.)
\end{enumerate}
\end{problem}

\begin{problem}\label{exer:7.1.19}  
Do the following experiment for various choices of
real numbers  $a_0$ and $a_1$.
\begin{enumerate}
\item % (a)
Use software  to solve the initial value problem
$$
(1+x)y''+2(x-1)^2y'+3y=0,\quad y(1)=a_0,\quad y'(1)=a_1,
$$
on the interval $(0,2)$. Choose the most accurate method
your software provides.
(See Section~10.1 for a brief discussion of one such
method.)
\item % (b)
For $N=2$, $3$, $4$, \dots, compute $a_2$, \dots, $a_N$
from Eqn.\eqref{eq:7.1.18} and graph
$$
T_N(x)=\sum_{n=0}^N a_nx^n
$$
and the solution obtained above on the same axes.
Continue increasing $N$ until it is obvious that there is
no point in continuing.
(This sounds vague, but you will know when to stop.)
\item Use Eqns.~\eqref{eq:7.1.24} and \eqref{eq:7.1.25}
to compute $\{a_n\}$.
\end{enumerate}
\end{problem}

\begin{problem}\label{exer:7.1.20}
Suppose the series $\sum_{n=0}^\infty a_nx^n$ converges on an
open interval $(-R,R)$, let $r$ be an arbitrary real number, and
define
$$
y(x)=x^r\sum_{n=0}^\infty a_nx^n=\sum_{n=0}^\infty a_nx^{n+r}
$$
on $(0,R)$. Use Theorem~\ref{thmtype:7.1.4} and the rule for
differentiating the product of two functions to show that
$$y'(x)=\sum_{n=0}^\infty  (n+r)a_nx^{n+r-1}$$
$$
y''(x)=\sum_{n=0}^\infty(n+r)(n+r-1)a_nx^{n+r-2}
$$
$$
\vdots
$$
$$
y^{(k)}(x)=\sum_{n=0}^\infty(n+r)(n+r-1)\cdots(n+r-k)a_nx^{n+r-k}
$$
on $(0,R)$

\begin{solution}
    $y'(x)=x^r\sum_{n=0}^\infty na_nx^{n-1}+rx^{r-1}\sum_{n=0}^\infty
a_nx^n=\sum_{n=0}^\infty (n+r)x^{n+r-1}$.

$$y''=\frac{d}{ dx}y'(x)=\frac{d}{ dx}\left[x^{r-1}\sum_{n=0}^\infty
(n+r)a_nx^n\right]=$$
$$=x^{r-1}\sum_{n=0}^\infty (n+r)na_nx^{n-1}+
(r-1)x^{r-2}\sum_{n=0}^\infty (n+r)a_nx^n=$$
$$=\sum_{n=0}^\infty
(n+r)(n+r-1)a_nx^{n+r-2}
$$
\end{solution}
\end{problem}

\begin{problem}\label{exer:7.1.21}
Let $y$ be as defined in Exercise~\ref{exer:7.1.20}, and write the given
expression in the form $x^r\sum_{n=0}^\infty b_nx^n$.

$x^2(1-x)y''+x(4+x)y'+(2-x)y$
\end{problem}

\begin{problem}\label{exer:7.1.22}
Let $y$ be as defined in Exercise~\ref{exer:7.1.20}, and write the given
expression in the form $x^r\sum_{n=0}^\infty b_nx^n$.

$x^2(1+x)y''+x(1+2x)y'-(4+6x)y$

\begin{solution}
    $$x^2(1+x)y''+x(1+2x)y'-(4+6x)y=$$
$$=(x^2y''+xy'-4y)+x(x^2y''+2xy'-6y)=$$
$$=\sum_{n=0}^\infty [(n+r)(n+r-1)+(n+r)-4]a_nx^{n+r}
+\sum_{n=0}^\infty [(n+r)(n+r-1)+2(n+r)-6]a_nx^{n+r+1}=$$
$$=\sum_{n=0}^\infty (n+r-2)(n+r+2)a_nx^{n+r}
+\sum_{n=0}^\infty (n+r+3)(n+r-2)a_nx^{n+r+1}=$$
$$=\sum_{n=0}^\infty (n+r-2)(n+r+2)a_nx^{n+r}
+\sum_{n=1}^\infty (n+r+2)(n+r-3)a_{n-1}x^{n+r}=$$
$$=x^r\sum_{n=0}^\infty  b_nx^n$$

with
$b_0=(r-2)(r+2)a_0$ and
$b_n=(n+r-2)(n+r+2)a_n+(n+r+2)(n+r-3)a_{n-1}$, $n\geq 1$.
\end{solution}
\end{problem}

\begin{problem}\label{exer:7.1.23}
Let $y$ be as defined in Exercise~\ref{exer:7.1.20}, and write the given
expression in the form $x^r\sum_{n=0}^\infty b_nx^n$.

$x^2(1+x)y''-x(1-6x-x^2)y'+(1+6x+x^2)y$
\end{problem}

\begin{problem}\label{exer:7.1.24}
Let $y$ be as defined in Exercise~\ref{exer:7.1.20}, and write the given
expression in the form $x^r\sum_{n=0}^\infty b_nx^n$.

$x^2(1+3x)y''+x(2+12x+x^2)y'+2x(3+x)y$

\begin{solution}
    $$x^2(1+3x)y''+x(2+12x+x^2)y'+2x(3+x)y=$$
$$=(x^2y''+2xy')+x(3x^2y''+12xy'+6y)+x^2(xy'+2y)=$$
$$=
\sum_{n=0}^\infty [(n+r)(n+r-1)+2(n+r)]a_nx^{n+r}
+\sum_{n=0}^\infty [3(n+r)(n+r-1)+12(n+r)+6]a_nx^{n+r+1}
+\sum_{n=0}^\infty[(n+r)+2]a_nx^{n+r+2 }=$$
$$=\sum_{n=0}^\infty (n+r)(n+r+1)a_nx^{n+r}
+3\sum_{n=0}^\infty (n+r+1)(n+r+2)a_nx^{n+r+1}
+\sum_{n=0}^\infty (n+r+2)a_nx^{n+r+2}=$$
$$=\sum_{n=0}^\infty (n+r)(n+r+1)a_nx^{n+r}
+3\sum_{n=1}^\infty (n+r)(n+r+1)a_{n-1}x^{n+r}
+\sum_{n=2}^\infty (n+r)a_{n-2}x^{n+r}=$$
$$=x^r\sum_{n=0}^\infty  b_nx^n$$
with
$b_0=r(r+1)a_0$,
$b_1=(r+1)(r+2)a_1+3(r+1)(r+2)a_0$,
$b_n=(n+r)(n+r+1)a_n+3(n+r)(n+r+1)a_{n-1}+(n+r)a_{n-2}$,
$n\geq 2$.

\end{solution}
\end{problem}

\begin{problem}\label{exer:7.1.25}
Let $y$ be as defined in Exercise~\ref{exer:7.1.20}, and write the given
expression in the form $x^r\sum_{n=0}^\infty b_nx^n$.

$x^2(1+2x^2)y''+x(4+2x^2)y'+2(1-x^2)y$
\end{problem}

\begin{problem}\label{exer:7.1.26}
Let $y$ be as defined in Exercise~\ref{exer:7.1.20}, and write the given
expression in the form $x^r\sum_{n=0}^\infty b_nx^n$.

$x^2(2+x^2)y''+2x(5+x^2)y'+2(3-x^2)y$

\begin{solution}
    $$x^2(2+x^2)y''+2x(5+x^2)y'+2(3-x^2)y=$$
$$=(2x^2y''+10xy'+6y)+x^2(x^2y''+2xy'-2y)=$$
$$=
\sum_{n=0}^\infty [2(n+r)(n+r-1)+10(n+r)+6]a_nx^{n+r}
+\sum_{n=0}^\infty [(n+r)(n+r-1)+2(n+r)-2]a_nx^{n+r+2}=$$
$$=2\sum_{n=0}^\infty (n+r+1)(n+r+3)a_nx^{n+r}
+\sum_{n=0}^\infty (n+r-1)(n+r+2)a_nx^{n+r+2}=$$
$$=2\sum_{n=0}^\infty (n+r+1)(n+r+3)a_nx^{n+r}
+\sum_{n=2}^\infty (n+r-3)(n+r)a_{n-2}x^{n+r}=$$
$$=x^r\sum_{n=0}^\infty  b_nx^n$$
with
$b_0=2(r+1)(r+3)a_0$,
$b_1=2(r+2)(r+4)a_1$
$b_n=2(n+r+1)(n+r+3)a_n+(n+r-3)(n+r)a_{n-2}$,
$n\geq 2$.
\end{solution}
\end{problem}

\end{document}