\documentclass{ximera}
\input{../preamble.tex}

\title{Exercises} \license{CC BY-NC-SA 4.0}

\begin{document}

\begin{abstract}
\end{abstract}
\maketitle

\begin{onlineOnly}
\section*{Exercises}
\end{onlineOnly}



\begin{problem}\label{exer:7.4.1} 
Find the general solution of
the given Euler equation on $(0,\infty)$.

$x^2y''+7xy'+8y=0$
\end{problem}

\begin{problem}\label{exer:7.4.2} 
Find the general solution of
the given Euler equation on $(0,\infty)$.

$x^2y''-7xy'+7y=0$

\begin{solution}
    $p(r)=r(r-1)-7r+7=(r-7)(r-1)$; $y=c_1x+c_2x^7$.
\end{solution}
\end{problem}


\begin{problem}\label{exer:7.4.3} 
Find the general solution of
the given Euler equation on $(0,\infty)$.

$x^2y''-xy'+y=0$
\end{problem}

\begin{problem}\label{exer:7.4.4} 
Find the general solution of
the given Euler equation on $(0,\infty)$.

$x^2y''+5xy'+4y=0$

\begin{solution}
    $p(r)=r(r-1)+5r+4=(r+2)^2$;$y=x^{-2}(c_1+c_2 \ln x)$
\end{solution}
\end{problem}

\begin{problem}\label{exer:7.4.5} 
Find the general solution of
the given Euler equation on $(0,\infty)$.

$x^2y''+xy'+y=0$
\end{problem}

\begin{problem}\label{exer:7.4.6} 
Find the general solution of
the given Euler equation on $(0,\infty)$.

$x^2y''-3xy'+13y=0$

\begin{solution}
    $p(r)=r(r-1)-3r+13=(r-2)^2+9$;
 $y=x^2[c_1 \cos (3 \ln x)+c_2 \sin (3 \ln x)]$.

\end{solution}
\end{problem}


\begin{problem}\label{exer:7.4.7} 
Find the general solution of
the given Euler equation on $(0,\infty)$.

$x^2y''+3xy'-3y=0$
\end{problem}

\begin{problem}\label{exer:7.4.8}
Find the general solution of
the given Euler equation on $(0,\infty)$.

$12x^2y''-5xy''+6y=0$

\begin{solution}
    $p(r)=12r(r-1)-5r+6=(3r-2)(4r-3)$;
$y=c_1x^{2/3}+c_2 x^{3/4}$.
\end{solution}
\end{problem}

\begin{problem}\label{exer:7.4.9} 
Find the general solution of
the given Euler equation on $(0,\infty)$.

$4x^2y''+8xy'+y=0$
\end{problem}

\begin{problem}\label{exer:7.4.10}
Find the general solution of
the given Euler equation on $(0,\infty)$.

$3x^2y''-xy'+y=0$

\begin{solution}
    $p(r)=3r(r-1)-r+1=(r-1)(3r-1)$; $y=c_1x+c_2x^{1/3}$.
\end{solution}
\end{problem}

\begin{problem}\label{exer:7.4.11} 
Find the general solution of
the given Euler equation on $(0,\infty)$.

$2x^2y''-3xy'+2y=0$
\end{problem}

\begin{problem}\label{exer:7.4.12}
Find the general solution of
the given Euler equation on $(0,\infty)$.

$x^2y''+3xy'+5y=0$

\begin{solution}
    $p(r)=r(r-1)+3r+5=(r+1)^2+4$;
$y=\frac
 {1}{ x}\left[c_1\cos(2 \ln x)+c_2\sin(2 \ln x\right]$
\end{solution}
\end{problem}

\begin{problem}\label{exer:7.4.13} 
Find the general solution of
the given Euler equation on $(0,\infty)$.

$9x^2y''+15xy'+y=0$
\end{problem}

\begin{problem}\label{exer:7.4.14}
Find the general solution of
the given Euler equation on $(0,\infty)$.

$x^2y''-xy'+10y=0$

\begin{solution}
    $p(r)=r(r-1)-r+10=(r-1)^2+9$;
 $y=x\left[c_1\cos(3 \ln x)+c_2\sin(3 \ln x)\right]$.
\end{solution}
\end{problem}

\begin{problem}\label{exer:7.4.15} 
Find the general solution of
the given Euler equation on $(0,\infty)$.

$x^2y''-6y=0$
\end{problem}

\begin{problem}\label{exer:7.4.16}
Find the general solution of
the given Euler equation on $(0,\infty)$.

$2x^2y''+3xy'-y=0$

\begin{solution}
    $p(r)=2r(r-1)+3r-1=(r+1)(2r-1)$;
$y=\frac{c_1}{ x}+c_2 x^{1/2}$.
\end{solution}
\end{problem}


\begin{problem}\label{exer:7.4.17} 
Find the general solution of
the given Euler equation on $(0,\infty)$.

$x^2y''-3xy'+4y=0$
\end{problem}

\begin{problem}\label{exer:7.4.18}
Find the general solution of
the given Euler equation on $(0,\infty)$.

$2x^2y''+10xy'+9y=0$

\begin{solution}
    $p(r)=2r(r-1)+10r+9=2(r+2)^2+1$;
    
$y=\frac{1}{ x^2}
\left[c_1\cos\left(\frac{1}{\sqrt{2}} \ln x\right)+c_2\sin
\left(\frac{1}{\sqrt{2}} \ln x\right) \right]$.
\end{solution}
\end{problem}

\begin{problem}\label{exer:7.4.19}
\begin{enumerate}
\item % (a)
Adapt the proof of Theorem~\ref{thmtype:7.4.3} to show that  $y=y(x)$
satisfies the Euler equation

\begin{equation} \label{eq:7.4.exer:7.4.19A}
ax^2y''+bxy'+cy=0
\end{equation}
on $(-\infty,0)$
if and only if  $Y(t)=y(-e^t)$
$$
a \frac{d^2Y}{ dt^2}+(b-a)\frac{dY}{ dt}+cY=0.
$$
on   $(-\infty,\infty)$.
\item % (b)
Use part (a)  to show that  the general solution of
\eqref{eq:7.4.exer:7.4.19A} on $(-\infty,0)$ is
\begin{eqnarray*}
y&=&c_1|x|^{r_1}+c_2|x|^{r_2}\mbox{ if $r_1$ and $r_2$ are distinct
real numbers;  }
\\ y&=&|x|^{r_1}(c_1+c_2\ln|x|)\mbox{ if
$r_1=r_2$;  }
\\ y&=&|x|^{\lambda}\left[c_1\cos\left(\omega\ln|x|\right)+
c_2\sin\left(\omega\ln|x| \right)\right]\mbox{ if
$r_1,r_2=\lambda\pm i\omega$ with $\omega>0$}.
\end{eqnarray*}
\end{enumerate}
\end{problem}

\begin{problem}\label{exer:7.4.20} Use reduction of order to show that if
$$
ar(r-1)+br+c=0
$$
has a repeated root $r_1$ then $y=x^{r_1}(c_1+c_2\ln x)$ is the
general solution of
$$
ax^2y''+bxy'+cy=0
$$
on $(0,\infty)$.

\begin{solution}
    If $p(r)=ar(r-1)+br+c=a(r-r_1)^2$, then (A) $p(r_1)=p'(r_1)=0$.
If $y=ux^{r_1}$, then $$y'=u'x^{r_1}+r_1ux^{r_1-1}$$
and $$y''=u''x^{r_1}+2r_1u'x_1^{r_1-1}+r_1(r_1-1)x_1^{r_1-2}$$ so
$$
ax^2y''+bxy'+cy=$$
$$=ax^{r_1+2}u''+(2ar_1+b)x^{r_1+1}u'
+\left(ar_1(r_1-1)+br_1+c\right)x^{r_1}u=$$
$$=ax^{r_1+2}u''+p'(r_1)x_1^{r_1+1}u'+p(r)x^{r_1}u=$$
$$=ax^{r_1+2}u''$$
from (A). Therefore, $u''=0$, so $u=c_1+c_2x$ and
$y=x^{r_1}(c_1+c_2x)$.
\end{solution}
\end{problem}

\begin{problem}\label{exer:7.4.21}
  A nontrivial solution of
$$
P_0(x)y''+P_1(x)y'+P_2(x)y=0
$$
is said to be \emph{oscillatory} on an interval $(a,b)$ if it has infinitely
many zeros on $(a,b)$.  Otherwise, $y$ is said to be \emph{nonoscillatory}
on $(a,b)$.  Show that the equation
$$
x^2y''+ky=0 \quad (k=\; \mbox{constant})
$$
has oscillatory solutions on $(0,\infty)$ if and only if $k>1/4$.
\end{problem}

\begin{problem}\label{exer:7.4.22}
In Example~\ref{example:7.4.2} we saw  that $x_0=1$ and $x_0=-1$
are regular singular points of Legendre's equation
$$
(1-x^2)y''-2xy'+\alpha(\alpha+1)y=0\quad
\text{(A)}
$$
\begin{enumerate}
\item % (a)
Introduce the new variables $t=x-1$  and $Y(t)=y(t+1)$, and show that
$y$  is a solution of (A) if and only if
$Y$ is a solution of
$$
t(2+t)\frac{d^2Y}{ dt^2}+2(1+t)\frac{dY}{ dt}-\alpha(\alpha+1)Y=0,
$$
which has a regular singular point at $t_0=0$.

\begin{solution}
    If $t=x-1$ and $Y(t)=y(t+1)=y(x)$, then
$$(1-x^2)y''-2xy'+\alpha(\alpha+1)y=$$
$$=-t(2+t)\frac{d^2Y}{ dt^2}-2(1+t)\frac{dY}{ dt}+\alpha(\alpha+1)Y=0$$
so $y$ satisfies Legendre's equation if and only if $Y$ satisfies

(A)\quad $t(2+t)\frac{d^2Y}{ dt^2}+2(1+t)\frac{dY}{
dt}-\alpha(\alpha+1)Y=0$. 

Since (A) can be rewritten as
$$t^2(2+t)\frac{d^2Y}{ dt^2}+2t(1+t)\frac{dY}{
dt}-\alpha(\alpha+1)tY=0$$ (A) has a regular singular point at
$t=0_0$.

\end{solution}

\item % (b)
Introduce the new variables $t=x+1$  and $Y(t)=y(t-1)$, and show that
$y$  is a solution of (A) if and only if
$Y$ is a solution of
$$
t(2-t)\frac{d^2Y}{ dt^2}+2(1-t)\frac{dY}{ dt}+\alpha(\alpha+1)Y=0,
$$
which has a regular singular point at $t_0=0$.

\begin{solution}
    If $t=x+1$ and $Y(t)=y(t-1)=y(x)$, then
$$(1-x^2)y''-2xy'+\alpha(\alpha+1)y=$$
$$=t(2-t)\frac{d^2Y}{ dt^2}+2(1-t)\frac{dY}{ dt}+\alpha(\alpha+1)Y$$
so $y$ satisfies Legendre's equation if and only if $Y$ satisfies

(B)\quad $t(2-t)\frac{d^2Y}{ dt^2}+2(1-t)\frac{dY}{
dt}+\alpha(\alpha+1)Y$,

 Since (B) can be rewritten as
 
$$t^2(2-t)\frac{d^2Y}{ dt^2}+2t(1-t)\frac{dY}{
dt}+\alpha(\alpha+1)tY$$

(B) has a regular singular point at
$t=0_0$.
\end{solution}
\end{enumerate}
\end{problem}

\begin{problem}\label{exer:7.4.23}
Let  $P_0,P_1$, and $P_2$ be polynomials  with no common factor,  and
suppose   $x_0\neq 0$ is a singular point of
$$
P_0(x)y''+P_1(x)y'+P_2(x)y=0\quad
\text{(A)}
$$
Let $t=x-x_0$ and $Y(t)=y(t+x_0)$.
\begin{enumerate}
\item % (a)
Show that $y$ is a solution of (A) if and only if $Y$
is a solution of
$$
R_0(t)\frac{d^2Y}{ dt^2}+R_1(t)\frac{dY}{ dt}+R_2(t)Y=0\quad
\text{(B)}
$$
where
$$
R_i(t)=P_i(t+x_0),\quad i=0,1,2.
$$
\item % (b)
Show that $R_0$, $R_1$, and $R_2$ are polynomials in $t$ with no common
factors, and $R_0(0)=0$; thus,  $t_0=0$ is a singular
point of (B).
\end{enumerate}
\end{problem}

\end{document}